crypto.v
@@ -1,0 +1,171 @@
+From mathcomp Require Import ssreflect.
+From iris.algebra Require Import excl auth frac agree gmap list.
+From iris.proofmode Require Import tactics.
+From iris.program_logic Require Import language.
+From iris.program_logic Require Import lifting.
+From iris.algebra Require Import gmap auth gset numbers excl agree ofe.
+From iris.heap_lang Require Import notation proofmode metatheory.
+From iris.heap_lang Require Import primitive_laws.
+From iris.base_logic.lib Require Import invariants.
+From iris_string_ident Require Import ltac2_string_ident.
+From crypto Require Import basic.
+
+Section Keys.
+
+Class keySG Σ := KeySG {
+  key_inG :> inG Σ (authR (gsetUR (prodO locO locO)));
+  key2_symbol : symbol_kind;
+  key1_symbol : symbol_kind;
+  key_name : gname;
+}.
+
+Context `{symbolSG Σ, keySG Σ}.
+
+Implicit Types LL : gsetUR (prodO locO locO).
+Implicit Types ll : prodO locO locO.
+Implicit Types Lb : gsetUR (prodO boolO locO).
+Implicit Types l : locO.
+
+Definition key_inv : iProp Σ :=
+  ∃ LL,
+    own key_name (● LL) ∗
+    ⌜perm LL⌝ ∗
+    ([∗ set] ll ∈ LL, symbol true  key2_symbol ll.1 ∗
+                      symbol false key2_symbol ll.2).
+
+Definition key l1 l2 : iProp Σ :=
+  own key_name (◯ {[l1, l2]}).
+
+Global Instance key_persistent l1 l2 : Persistent (key l1 l2).
+Proof. apply _. Qed.
+
+Lemma key_permR l1 l21 l22 :
+  key_inv -∗ key l1 l21 -∗ key l1 l22 -∗ ⌜l21 = l22⌝.
+Proof.
+iDestruct 1 as (LL) "(Hown & %Hperm & Halloc)".
+iIntros "Hl21 Hl22"; rewrite /key.
+iPoseProof (own_valid_2 with "Hown Hl21") as "%Hvalid1".
+rewrite auth_both_valid in Hvalid1 *; case=> Hvalid1 _.
+iPoseProof (own_valid_2 with "Hown Hl22") as "%Hvalid2".
+rewrite auth_both_valid in Hvalid2 *; case=> Hvalid2 _.
+have {}Hvalid1: (l1, l21) ∈ LL.
+  move/gset_included in Hvalid1; apply: Hvalid1.
+  by apply elem_of_singleton_2.
+have {}Hvalid2: (l1, l22) ∈ LL.
+  move/gset_included in Hvalid2; apply: Hvalid2.
+  by apply elem_of_singleton_2.
+by iPureIntro; apply (Hperm _ _ Hvalid1 Hvalid2).
+Qed.
+
+Lemma key_permL l11 l12 l2 :
+  key_inv -∗ key l11 l2 -∗ key l12 l2 -∗ ⌜l11 = l12⌝.
+Proof.
+iDestruct 1 as (LL) "(Hown & %Hperm & Halloc)".
+rewrite /key; iIntros "Hl11 Hl12".
+iPoseProof (own_valid_2 with "Hown Hl11") as "%Hvalid1".
+iPoseProof (own_valid_2 with "Hown Hl12") as "%Hvalid2".
+move: Hvalid1; rewrite auth_both_valid; case=> Hvalid1 _.
+move: Hvalid2; rewrite auth_both_valid; case=> Hvalid2 _.
+have {}Hvalid1 : (l11, l2) ∈ LL.
+  move/gset_included in Hvalid1; apply: Hvalid1.
+  by apply elem_of_singleton_2.
+have {}Hvalid2 : (l12, l2) ∈ LL.
+  move/gset_included in Hvalid2; apply: Hvalid2.
+  by apply elem_of_singleton_2.
+by iPureIntro; apply (Hperm _ _ Hvalid1 Hvalid2).
+Qed.
+
+End Keys.
+
+Section Terms.
+
+Context `{heapG Σ, cfgSG Σ, symbolSG Σ}.
+
+Implicit Types s : side.
+
+Definition lo_nonce : symbol_kind := 1%positive.
+Definition hi_nonce : symbol_kind := 2%positive.
+Definition lo_key   : symbol_kind := 3%positive.
+Definition hi_key   : symbol_kind := 4%positive.
+
+Inductive term  :=
+| TInt of Z
+| TPair of term & term
+| TNonce of loc
+| TKey of loc
+| TEnc of loc & term.
+
+Fixpoint val_of_term t : val :=
+  match t with
+  | TInt n => (#0, #n)
+  | TPair t1 t2 => (#1, (val_of_term t1, val_of_term t2))%V
+  | TNonce l => (#2, #l)%V
+  | TKey l => (#3, #l)%V
+  | TEnc l t => (#4, (#l, val_of_term t))
+  end.
+
+
+Class termSG := TermSG {
+  term_inG  :> inG Σ (authR (gsetUR (prodO valO valO)));
+  term_name :  gname
+}.
+
+Section Terms.
+
+Context `{termSG}.
+
+Fixpoint opaque s t : iProp Σ :=
+  match t with
+  | TInt _ => False%I
+  | TPair _ _ => False%I
+  | TNonce l => symbol s lo_nonce l
+  | TKey l => False%I
+  | TEnc l t => symbol s hi_key l
+  end.
+
+Implicit Types TT : gsetUR (prodO valO valO).
+
+Definition opaque_inv : iProp Σ :=
+  ∃ TT, own term_name (● TT)
+        ∗ (∀ v1 v2, ⌜(v1, v2) ∈ TT⌝ -∗
+           ∃ t1 t2, ⌜v1 = val_of_term t1⌝ ∗
+                    ⌜v2 = val_of_term t2⌝ ∗
+                    opaque Left t1 ∗ opaque Right t2).
+
+Fixpoint lo_term' t1 t2 : iProp Σ :=
+  own term_name (◯ {[val_of_term t1, val_of_term t2]}) ∨
+  match t1, t2 with
+  | TInt n1, TInt n2 => ⌜n1 = n2⌝
+  | TPair t11 t12, TPair t21 t22 =>
+    lo_term' t11 t21 ∗ lo_term' t12 t22
+  | TNonce l1, TNonce l2 =>
+    symbol lo_nonce #l1 #l2
+  | TKey l1, TKey l2 =>
+    symbol lo_key #l1 #l2
+  | TEnc l1 t1, TEnc l2 t2 =>
+    symbol lo_key #l1 #l2 ∗ lo_term' t1 t2
+  | _, _ => False%I
+  end.
+
+
+
+
+Definition ty_nonce v1 v2 : iProp Σ :=
+  symbol lo_nonce v1 v2 ∨ symbol hi_nonce v1 v2.
+
+Definition ty_hi_nonce v1 v2 : iProp Σ :=
+  symbol hi_nonce v1 v2.
+
+Definition ty_key v1 v2 : iProp Σ :=
+  symbol lo_key v1 v2 ∨ symbol hi_key v1 v2.
+
+Definition ty_hi_key v1 v2 : iProp Σ :=
+  symbol hi_key v1 v2.
+
+Definition ty1 (ty : val → val → iProp Σ) left v : iProp Σ :=
+  ∃ v', if left then ty v v' else ty v' v.
+
+Definition ty_key1 := ty1 ty_key.
+Definition ty_hi_key1 := ty1 ty_hi_key.
+Definition ty_nonce1 := ty1 ty_nonce.
+Definition ty_hi_nonce1 := ty1 ty_hi_nonce.
